Language_Components/Calc/Calc_Mem_Imp_Hoare.thy
@@ -1,17 +1,137 @@
 theory Calc_Mem_Imp_Hoare
-  imports Calc_Mem_Imp "../../Hoare/Hoare_Direct_Dominant" "../../Hoare/Hoare_Lift"
+  imports Calc_Mem_Imp "../../Hoare/Hoare_Direct_Dominant" "../../Hoare/Hoare_Lift" "../Mem/Mem_Simple"
 begin
 
 (* Deriving a set of Hoare logic rules useful for reasoning about imperative code in Imp.
  * then, proceeding with an example.
  *)
 
-(* arith *)
+abbreviation sems where
+"sems \<equiv> {calc_sem_l, mem_sem_l, cond_sem_l, imp_sem_l, seq_sem_l}"
 
-(* cond *)
+abbreviation sems_nos where
+"sems_nos \<equiv> {calc_sem_l, mem_sem_l, cond_sem_l, imp_sem_l}"
 
-(* mem *)
+definition sem_final' :: "syn \<Rightarrow> ('s, _) state \<Rightarrow> ('s, _) state" where
+"sem_final' =
+  pcomps [calc_sem_l, mem_sem_l, cond_sem_l, imp_sem_l, seq_sem_l]"
 
-(* seq, imp: use as is *)
+
+lemma pres :
+"sups_pres sems"
+  sorry
+
+lemma calc_dom :
+  "\<And> c . calc_sem_l \<downharpoonleft> sems_nos (Sc c)"
+  sorry
+
+lemma cond_dom :
+  "\<And> b . cond_sem_l \<downharpoonleft> sems_nos (Sb b)"
+  sorry
+
+lemma mem_dom :
+  "\<And> m . mem_sem_l \<downharpoonleft> sems_nos (Sm m)"
+  sorry
+
+lemma seq_dom :
+  "\<And> s . seq_sem_l \<downharpoonleft> sems (Ss s)"
+  sorry
+
+lemma imp_dom :
+  "\<And> i . imp_sem_l \<downharpoonleft> sems (Si i)"
+  sorry
+
+
+definition start_state :: "syn gensyn \<Rightarrow> (syn, unit) Mem_Simple.state" where
+"start_state prog =
+  ( Swr [prog]
+  , mdp 0 None
+  , Swr 0, Swr 0, Swr 0, Swr 0
+  , empty
+  , ())"
+
+definition prog_mini :: "syn gensyn" where
+"prog_mini =  G (Sc (Cnum 42)) []
+"
+
+(* first test: a simple arithmetic *)
+definition prog0 :: "syn gensyn" where
+"prog0 =
+  G (Ss Sseq)
+  [ G (Sc (Cnum 42)) []
+  , G (Sm (Swrite (STR ''A'') Reg_c)) []
+  ]"
+
+definition prog00 :: "syn gensyn" where
+"prog00 =
+  G (Sb (Seqz)) []
+  "
+
+
+(* multiplication as repeated addition *)
+(* start with c = 0
+ * add arg1 to c
+ * decrement arg2 *)
+
+definition prog1 :: "int \<Rightarrow> int \<Rightarrow> syn gensyn" where
+"prog1 i1 i2 =
+  G (Ss Sseq)
+  [ G (Sc (Cnum i1)) []
+  , G (Sm (Swrite (STR ''arg1'') (Reg_c))) []
+  , G (Sc (Cnum i2)) []
+  , G (Sm (Swrite (STR ''arg2'') (Reg_c))) []
+  , G (Sc (Cnum 1)) []
+  , G (Sm (Swrite (STR ''one'') (Reg_c))) []
+  , G (Sc (Cnum 0)) []
+  , G (Sm (Swrite (STR ''acc'') (Reg_c))) []
+
+  , G (Sm (Sread (STR ''arg2'') (Reg_c))) []
+  , G (Sb Sgtz) []
+
+  , G (Si SwhileC)
+    [ G (Ss Sseq)
+      [G (Sm (Sread (STR ''arg1'') (Reg_a))) []
+      , G (Sm (Sread (STR ''acc'') (Reg_b))) []
+      , G (Sc Cadd) []
+      , G (Sm (Swrite (STR ''acc'') (Reg_c))) []
+      , G (Sm (Sread (STR ''arg2'') (Reg_a))) []
+      , G (Sm (Sread (STR ''one'') (Reg_b))) []
+      , G (Sc Csub) []
+      , G (Sm (Swrite (STR ''arg2'') (Reg_c))) []
+      , G (Sm (Sread (STR ''arg2'') (Reg_c))) []
+      , G (Sb Sgtz) []
+      ]
+    ]
+  ]
+"
+value "sem_run sem_final 100 (start_state prog0)"
+
+(* calc_sem_l and cond_sem_l
+*)
+value "sem_run (pcomps [calc_sem_l, mem_sem_l, seq_sem_l, cond_sem_l]) 100 (start_state prog_mini)"
+
+
+value "sem_run sem_final 100 (start_state prog_mini)"
+
+value "sem_run sem_final 100 (start_state (prog1 2 3))"
+
+  
+
+(* ok great - so this finally works. now let's see if we can prove anything. *)
+
+declare [[show_types = false]]
+declare [[show_sorts = false]]
+
+lemma prog1_spec :
+  assumes Hi1 : "0 \<le> i1"
+  assumes Hi2 : "0 \<le> i2"
+
+shows "|sem_final| {~ (\<lambda> _ . True) ~}
+                   [prog1 i1 i2]
+                   {~ (\<lambda> st . 
+                      (case st of
+                        (x0, x1, reg_flag, reg_c, reg_a, reg_b, mem, xz) \<Rightarrow>
+                          \<exists> p . get mem (STR ''acc'') = Some (mdp p (Some (mdt (i1 * i2))))))
+  ~}"
 
 end
