Language_Components/Calc/Calc_Mem_Hoare_Simp.thy
@@ -1,0 +1,175 @@
+theory Calc_Mem_Hoare
+  imports Calc Calc_Mem "../../Hoare/Hoare_Direct" "../../Hoare/Hoare_Lift" "../../Lifter/Auto_Lifter_Proofs"
+
+begin
+
+(* Hoare rule for Calc_Mem (integrated, for now - should be possible to explore
+ * separate Calc and Mem rules and composing them - TODO)
+ *)
+
+lemma HCalc_calc :
+  assumes Hc : "c \<noteq> Cskip"
+  shows "Calc.calc_sem % {{P1}} c
+                         {{(\<lambda> st . case st of
+                              (x1, x2, x3) \<Rightarrow> 
+                              (\<exists> x3' . P1 (x1, x2, x3')) \<and>
+                              (\<forall> x3' . calc_sem c (x1, x2, x3') = st))}}"
+proof(rule HTSI)
+  fix a
+  assume H : "P1 a"
+
+  show "case calc_sem c a of (x1, x2, x3) \<Rightarrow> (\<exists>x3'. P1 (x1, x2, x3')) \<and> (\<forall>x3'. calc_sem c (x1, x2, x3') = calc_sem c a)"
+    using Hc H
+    by(cases c; cases a; auto simp add: split: prod.splits)
+qed
+
+lemma HCalc_skip :
+  shows "Calc.calc_sem % {{P1}} Cskip
+                         {{P1}}"
+proof(rule HTSI)
+  fix a
+  assume H : "P1 a"
+
+  show "P1 (calc_sem Cskip a)"
+    using H
+    by(cases a; auto simp add: split: prod.splits)
+qed
+
+
+lemma HMem0_lit :
+  shows "mem0_sem % {{P1}} Slit s i
+                    {{(\<lambda> st . case st of (x1, x2) \<Rightarrow> (\<exists> x2' . P1 (x1, x2')) \<and> x2 = i)}}"
+proof(rule HTSI)
+  fix a
+  assume H : "P1 a"
+  show "case mem0_sem (Slit s i) a of (x1, x2) \<Rightarrow> (\<exists>x2'. P1 (x1, x2')) \<and> x2 = i" using H
+    by(cases a; auto)
+qed
+
+lemma HMem0_copy :
+  shows "mem0_sem % {{P1}} Scopy s1 s2
+                    {{(\<lambda> st . case st of (x1, x2) \<Rightarrow> (\<exists> x2' . P1 (x1, x2')) \<and> x2 = x1)}}"
+proof(rule HTSI)
+  fix a
+  assume H : "P1 a"
+  show "case mem0_sem (Scopy s1 s2) a of (x1, x2) \<Rightarrow> (\<exists>x2'. P1 (x1, x2')) \<and> x2 = x1" using H
+    by(cases a; auto)
+qed
+
+lemma HMem0_skip :
+  shows "mem0_sem % {{P1}} Mem.Sskip
+                    {{P1}}"
+proof(rule HTSI)
+  fix a
+  assume H : "P1 a"
+
+  show "P1 (mem0_sem Sskip a)"
+    using H
+    by(cases a; auto simp add: split: prod.splits)
+qed
+
+term "(schem_lift (SP NA NB)
+                (SM (SL mem_key_src (SPRI (SO NA)))
+                    (SL mem_key_dest (SPRIN 2 (SO NB)))))"  
+
+(* idea: now we need to say the dummy variable must already exist. *)
+(* we need to reevaluate how we are approaching ordering in the context of
+ * these lists...
+ *)
+lemma Mem_lift_valid :
+  shows "lifting_valid (schem_lift (SP NA NB)
+                (SM (SL mem_key_src (SPRI (SO NA)))
+                    (SL mem_key_dest (SPRIN 2 (SO NB)))) :: (Mem.syn, Mem.state0, Mem.state) lifting) 
+(\<lambda> syn . 
+  (case syn of
+    Slit s i \<Rightarrow> {st . (\<exists> s1v s1p . get st s1  = Some (mdp s1p (Some (mdt s1v)))) \<and> (\<exists> s0v s0p . get st (STR '''') = Some (mdp s0p (Some (mdt s0v))))}
+    | Scopy s1 s2 \<Rightarrow> {st . (\<exists> s1v s1p . get st s1  = Some (mdp s1p (Some (mdt s1v)))) \<and> (\<exists> s0v s0p . get st (STR '''') = Some (mdp s0p (Some (mdt s0v))))}
+    | _ \<Rightarrow> UNIV))"
+proof(rule lifting_validI)
+  fix s :: "Mem.syn" 
+  fix a :: "(int * int)"
+  fix b :: "Mem.state"
+  show "LOut (schem_lift (SP NA NB) (SM (SL mem_key_src (SPRI (SO NA))) (SL mem_key_dest (SPRC (\<lambda>_. 2) (SO NB))))) s
+        (LUpd (schem_lift (SP NA NB) (SM (SL mem_key_src (SPRI (SO NA))) (SL mem_key_dest (SPRC (\<lambda>_. 2) (SO NB))))) s a b) =
+       a"
+    apply(cases a; auto simp add: schem_lift_defs merge_l_def oalist_l_def prio_l_def option_l_def triv_l_def Let_def)
+     
+apply(cases "get b (mem_key_src s)"; auto simp add: get_update LNew_def prio_l_def)
+      apply(cases s; auto simp add: schem_lift_defs merge_l_def oalist_l_def prio_l_def option_l_def triv_l_def LNew_def split: option.split_asm)
+    term "SPR"
+    apply(auto split: sprio.splits simp add: prio_l_def schem_lift_defs)
+    apply(simp add: get_update)
+
+
+
+lemma HMem_lit : 
+  shows "Mem.mem_sem % {{P1}} (Slit s i)
+                       {{(\<lambda> st . 
+                          \<exists> st0 . P1 st0 \<and> st = update s i st0)}}"
+
+lemma HMem_copy : 
+  shows "Mem.mem_sem % {{P1}} c
+                       {{(\<lambda> st . True)}}"
+
+lemma HMem_skip : 
+  shows "Mem.mem_sem % {{P1}} c
+                       {{(\<lambda> st . True)}}"
+
+
+
+(* separate calc + mem rules, then merge (?). *)
+
+(* issue - need to deal with the fact that we might get default values back
+ * when things are not initialized. *)
+lemma HCalc_Mem_Calc :
+  shows "Calc_Mem.sem_final % {{P1}} (Sc calci s1 s2 s3) 
+                              {{(\<lambda> st . \<forall> v1 v2 v3 p1 p2 p3 . 
+                                (get st s1 = Some (mdp p1 (Some (mdt v1))) \<longrightarrow>
+                                (get st s2 = Some (mdp p2 (Some (mdt v2)))) \<longrightarrow>
+                                (get st s3 = Some (mdp p3 (Some (mdt v3)))) \<longrightarrow>
+                                ((\<forall> orig' . calc_sem calci (v1, v2, orig') = (v1, v2, v3))) \<and>
+                                 (\<exists> orig . P1 (update s3 orig st) \<or> P1 (delete s3 st)))) }}"
+proof(rule HTSI)
+  fix st
+  assume H: "P1 st"
+
+  show "\<forall>v1 v2 v3 p1 p2 p3.
+            get (sem_final (Sc calci s1 s2 s3) st) s1 = Some (mdp p1 (Some (mdt v1))) \<longrightarrow>
+            get (sem_final (Sc calci s1 s2 s3) st) s2 = Some (mdp p2 (Some (mdt v2))) \<longrightarrow>
+            get (sem_final (Sc calci s1 s2 s3) st) s3 = Some (mdp p3 (Some (mdt v3))) \<longrightarrow>
+            (\<forall>orig'. calc_sem calci (v1, v2, orig') = (v1, v2, v3)) \<and>
+            (\<exists>orig. P1 (update s3 orig (sem_final (Sc calci s1 s2 s3) st)) \<or> P1 (delete s3 (sem_final (Sc calci s1 s2 s3) st)))"
+  proof(step+)
+    fix v1 v2 v3 p1 p2 p3 orig'
+
+    assume Get1 : "get (sem_final (Sc calci s1 s2 s3) st) s1 = Some (mdp p1 (Some (mdt v1)))"
+    assume Get2 : "get (sem_final (Sc calci s1 s2 s3) st) s2 = Some (mdp p2 (Some (mdt v2)))"
+    assume Get3 : "get (sem_final (Sc calci s1 s2 s3) st) s3 = Some (mdp p3 (Some (mdt v3)))"
+
+    obtain r1 where Get1' : "get st s1 = Some r1" sorry
+    obtain r2 where Get2' : "get st s2 = Some r2" sorry
+    obtain r3 where Get3' : "get st s3 = Some r3" sorry
+
+    show "calc_sem calci (v1, v2, orig') = (v1, v2, v3)" using Get1 Get2 Get3
+      
+      apply(auto simp add: sem_final_def calc_sem_l_def mem_sem_l_def
+schem_lift_defs calc_key_lift_def merge_l_def oalist_l_def prio_l_def
+prod_bsup option_bsup bsup_oalist
+split: prod.splits
+)
+      apply(auto simp add: Get1' Get2' Get3' get_update)
+    
+
+  show "\<exists>v1 v2 v3 p1 p2 p3.
+            (get (sem_final (Sc calci s1 s2 s3) a) s1 = Some (mdp p1 (Some (mdt v1))) \<and>
+             get (sem_final (Sc calci s1 s2 s3) a) s2 = Some (mdp p2 (Some (mdt v2))) \<and>
+             get (sem_final (Sc calci s1 s2 s3) a) s3 = Some (mdp p3 (Some (mdt v3))) \<and> 
+             (\<forall>orig'. calc_sem calci (v1, v2, orig') = (v1, v2, v3))) \<and>
+            (\<exists>orig. P1 (update s3 orig (sem_final (Sc calci s1 s2 s3) a)) \<or>
+                    P1 (delete s3 (sem_final (Sc calci s1 s2 s3) a)))"
+
+
+    apply(auto simp add: calc_sem_l_def schem_lift_defs calc_key_lift_def merge_l_def oalist_l_def
+        )
+
+end
